% 01.tex
% Benjamin Davies
% 2017 02 08

\begin{enumerate}

	\item
	Find the first and second derivatives of the following functions.
	%
	\begin{enumerate}

		\item
		$a(x)=\ln(x^2)$.
		%
		\begin{solution}
			By the chain rule, the first derivative
			%
			\begin{align}
				a'(x)
				&= \frac{2x}{x^2}\\
				&= \frac{2}{x}
			\end{align}
			%
			and the second derivative
			\[ a''(x)=-\frac{2}{x^2}. \]
		\end{solution}

		\item
		$b(x)=x\ln(x)$.
		%
		\begin{solution}
			By the product rule, the first derivative
			%
			\begin{align}
				b'(x)
				&= \ln(x)+\frac{x}{x}\\
				&= \ln(x)+1
			\end{align}
			%
			and the second derivative
			\[ b''(x)=\frac{1}{x}. \]
		\end{solution}

		\item
		$c(x)=(\ln(x))^2$.
		%
		\begin{solution}
			By the chain rule, the first derivative
			\[ c'(x)=\frac{2\ln(x)}{x}. \]
			%
			By the quotient rule, the second derivative
			%
			\begin{align}
				c''(x)
				&= \frac{(2/x)x-2\ln(x)}{x^2}\\
				&= \frac{2-2\ln(x)}{x^2}.
			\end{align}
		\end{solution}

	\end{enumerate}

	\item
	Let~$f(x)$ be an arbitrary function with~$x\in\R$.
	Find the first and second derivatives of the following functions.
	%
	\begin{enumerate}

		\item
		$a(x)=f(x^2)$.
		%
		\begin{solution}
			By the chain rule, the first derivative
			\[ a'(x)=2xf'(x^2). \]
			By the product and chain rules, the second derivative
			\[ a''(x)=2f'(x^2)+4x^2f''(x^2). \]
		\end{solution}

		\item
		$b(x)=(f(x))^2$.
		%
		\begin{solution}
			By the chain rule, the first derivative
			\[ b'(x)=2f'(x)f(x). \]
			By the product rule, the second derivative
			\[ b''(x)=2f''(x)f(x)+2(f'(x))^2. \]
		\end{solution}

		\item
		$c(x)=f(\sqrt{x})$.
		%
		\begin{solution}
			By the chain rule, the first derivative
			\[ c'(x)=\frac{f'(\sqrt{x})}{2\sqrt{x}}. \]
			By the quotient rule, the second derivative
			%
			\begin{align}
				c''(x)
				&= \frac{(f''(\sqrt{x})/2\sqrt{x})2\sqrt{x}%
					-f'(\sqrt{x})/\sqrt{x}}{4x}\\
				&= \frac{f''(\sqrt{x})\sqrt{x}-f'(\sqrt{x})}{4x^{3/2}}.
			\end{align}
		\end{solution}

		\item
		$d(x)=\sqrt{f(x)}$.
		%
		\begin{solution}
			By the chain rule, the first derivative
			\[ d'(x)=\frac{f'(x)}{2\sqrt{f(x)}}. \]
			By the quotient rule, the second derivative
			%
			\begin{align}
				d''(x)
				&= \frac{2f''(x)\sqrt{f(x)}-2f'(x)(f'(x)/2\sqrt{f(x)})}%
					{4f(x)}\\
				&= \frac{2f(x)f''(x)-(f'(x))^2}{4(f(x))^{3/2}}.
			\end{align}
		\end{solution}

	\end{enumerate}

\end{enumerate}
